<subsection xmlns:xi="http://www.w3.org/2001/XInclude" xml:id="subsec-polar-form-of-a-complex">
<title> Polar form of a complex number</title>
<definition xml:id="def-polar-form-of-a-complex">
    <statement>
        <p>
            Let <m>r</m> and <m>\theta</m> be polar coordinates of the point (x, y) of the complex number <m>z = x+iy</m>. Since x = <m>r\text{cos}\theta</m>and y = <m>r\text{sin}\theta</m>, then the complex number can be written as : <m>\underline{\underline{\ z = r(\text{cos}\theta + i\text{sin}\theta)}}</m> which is called polar form, where <m>r</m> is modulus of <m>z</m> and <m>\ \theta\ </m>is principal argument of <m>z</m>.
        </p>
    </statement>
</definition>

<example>
    <statement>
        <p>
            Express the following complex numbers in polar form:
        </p>
        <p>
            <m>a)\ z = 1 + i </m>
        </p>
        <p>
            <m>\text{solution}:\ r = \sqrt{2}\ \text{and}\ \theta = \text{tan}^{- 1}(1) = \frac{\pi}{4} \text{.}</m>
        </p>
        <p>
            <m>\ \text{Thus},\ z = \sqrt{2}(\text{cos} \frac{\pi}{4} + i\text{sin} \frac{\pi}{4})\text{.}</m>
        </p>
        <p>
            <m>b)\ z = 3 - 3i\ \text{solution}:\ r = \sqrt{18}\ \text{and}\ \theta = \text{tan}^{- 1}( - 1) = - \frac{\pi}{4}\text{.}</m>
        </p>
        <p>
            <m>\text{solution}: \ r = \sqrt{\text{18}}\ \text{and}\ \theta = \text{tan}^{- 1}( - 1) = - \pi 4\text{.}\  \\</m>
        </p>
        <p>
            <m>\text{Thus},\ z = \sqrt{\text{18}}(\text{cos} - \frac{\pi}{4} + i\text{sin} - \frac{\pi}{4}) = \sqrt{\text{18}}(\text{cos}\frac{\pi}{4} - i\text{sin}\frac{\pi}{4})\text{.} \\</m>
        </p>
    </statement>
</example>

<p>
    <me>\textbf{Multiplication and division in polar forms}</me>
</p>
<p>
    <m>\text{If} \ z_{1}\ = r_{1}(\text{cos}\theta_{1} + i\text{sin}\theta_{1}) \ \ \ \text{and} \ \ \ \ z_{2} = r_{2}(\text{cos}\theta_{2} + i\text{sin}\theta_{2}), \text{then}</m>
</p>
<p>
    <m>a) \ \ z_{1} \cdot z_{2} = r_{1} \cdot r_{2}(\text{cos}(\theta_{1} + \theta_{2}) + i\text{sin}(\theta_{1} + \theta_{2}))</m>
</p>
<p>
    <m>b) \ \ \frac{z_{1}}{z_{2}} = \frac{r_{1}} {r_{2}}(\text{cos}(\theta_{1} - \theta_{2}) + i\text{sin}(\theta_{1} - \theta_{2}))</m>.
</p>
<p>
    <m>\textbf{Proof:}</m>
</p>
<p>
    <m>\text{a)} \ z_{1} \cdot z_{2} = r_{1}(\text{cos}\theta_{1} + i\text{sin}\theta_{1}) \cdot r_{2}(\text{cos}\theta_{2} + i\text{sin}\theta_{2})</m>
</p>
<p>
    <m> \ \ \ \ \ \ \ \ \ \ \ = r_{1} \cdot r_{2} \left [ \text{cos}\theta_{1}(\text{cos}\theta_{2} + i\text{sin}\theta_{2}) + i\text{sin}\theta_{1}(\text{cos}\theta_{2} + i\text{sin}\theta_{2}) \right ]</m>
</p>
<p>
    <m> \ \ \ \ \ \ \ \ \ \ \ = r_{1} \cdot r_{2} \left [ \text{cos}\theta_{1}\text{cos}\theta_{2} + i\text{cos}\theta_{1}\text{sin}\theta_{2} + i\text{sin}\theta_{1}\text{cos}\theta_{2} - \text{sin}\theta_{1}\text{sin}\theta_{2} \right ]</m>
</p>
<p>
    <m> \ \ \ \ \ \ \ \ \ \ \ = r_{1} \cdot r_{2} \left [ \text{cos}\theta_{1}\text{cos}\theta_{2} - \text{sin}\theta_{1}\text{sin}\theta_{2} + i(\text{cos}\theta_{1}\text{sin}\theta_{2} + \text{sin}\theta_{1}\text{cos}\theta_{2}) \right ]</m>
</p>
<p>
    <m> \ \ \ \ \ \ \ \ \ \ \ = \underline{\underline{ r_{1} \cdot r_{2} \left [ \text{cos}(\theta_{1} + \theta_{2}) + i \ \text{sin}(\theta_{1} + \theta_{2})\right ]}}</m>
</p>
<p>
    <m>\text{Thus,} \ z_{1} \cdot z_{2} = r_{1} \cdot r_{2}(\text{cos}(\theta_{1} + \theta_{2}) + i \ \text{sin}(\theta_{1} + \theta_{2}))</m>
</p>

<p>
    <m>\text{b)} \ \frac{z_{1}}{z_{2}} = \frac{r_{1} (\text{cos}\theta_{1} + i\text{sin}\theta_{1})}{ r_{2} (\text{cos}\theta_{2} + i\text{sin}\theta_{2})} = \frac{r_{1}}{r_{2}} \left ( \frac{\text{cos}\theta_{1} + i\text{sin}\theta_{1}}{\text{cos}\theta_{2} + i\text{sin}\theta_{2}} \right )</m>
</p>
<p>
    <m> \ \ \ \ \ \ \ \ = \frac{r_{1}}{r_{2}} \left ( \frac{\text{cos}\theta_{1} + i\text{sin}\theta_{1}}{\text{cos}\theta_{2} + i\text{sin}\theta_{2}} \right ) \cdot \frac{\text{cos}\theta_{2} - i\text{sin}\theta_{2}}{\text{cos}\theta_{2} - i\text{sin}\theta_{2}}</m>
</p>
<p>
    <m> \ \ \ \ \ \ \ \ = \frac{r_{1}}{r_{2}} \left ( \frac{ \text{cos}\theta_{1}\text{cos}\theta_{2} - i\text{cos}\theta_{1}\text{sin}\theta_{2} + i\text{sin}\theta_{1}\text{cos}\theta_{2} + \text{sin}\theta_{1}\text{sin}\theta_{2} }{\text{cos}^{2}\theta_{2} + \text{sin}^{2}\theta_{2}}\right )</m>
</p>
<p>
    <m> \ \ \ \ \ \ \ \ = \frac{r_{1}}{r_{2}} \left ( \frac{\text{cos}\theta_{1}\text{cos}\theta_{2} + \text{sin}\theta_{1}\text{sin}\theta_{2} + i(\text{sin}\theta_{1}\text{cos}\theta_{2} - \text{cos}\theta_{1}\text{sin}\theta_{2})}{1} \right )</m> 
</p>
<p>
    <m> \ \ \ \ \ \ \ \ = \underline{\underline{ \frac{r_{1}}{r_{2}} \left [ \text{cos}(\theta_{1} - \theta_{2}) + i\text{sin}(\theta_{1} - \theta_{2})\right ]}}</m>
</p>
<p>
    <m>\text{Thus,} \ \frac{z_{1}}{z_{2}} = \frac{r_{1}}{r_{2}}(\text{cos}(\theta_{1} - \theta_{2}) + i\text{sin}(\theta_{1} - \theta_{2}))</m>
</p>

<example>
    <statement>
        <p>
            If <m>z_{1} = 6(\text{cos}\frac{\pi}{2} + i\text{sin} \frac{\pi}{2})</m> and <m>z_{2} = 2(\text{cos}\frac{\pi}{3} + i\text{sin}\frac{\pi}{3})</m>, then find:
        </p>
        <p>
            <m>a) \ z_{1} \cdot z_{2} \ \ \ \ \ b) \ \frac{z_{1}}{z_{2}}</m>
        </p>
    </statement>
    <solution>
        <p>
            <m>\text{a) } z_{1} \cdot z_{2} = 6 \cdot 2 \left [ \text{cos}\left(\frac{\pi}{2} + \frac{\pi}{3}\right) + i\text{sin}\left(\frac{\pi}{2} + \frac{\pi}{3}\right) \right ]</m>
        </p>
        <p>
            <m> \ \ \ \ \ \ \ \ = \underline{\underline{ 12\left [ \text{cos}\left(\frac{5\pi}{6}\right) + i\text{sin}\left(\frac{5\pi}{6}\right) \right ]}}</m>
        </p>
        <p>
            <m>\text{b) } \frac{z_{1}}{z_{2}} = \frac{6}{2} \left [ \text{cos}\left(\frac{\pi}{2} - \frac{\pi}{3}\right) + i\text{sin}\left(\frac{\pi}{2} - \frac{\pi}{3}\right) \right ]</m>
        </p>
        <p>
            <m> \ \ \ \ \ \ \ \ = \underline{\underline{ 3\left [ \text{cos}\left(\frac{\pi}{6}\right) + i\text{sincos}\left(\frac{\pi}{6}\right) \right ]}}</m>
        </p>
        <p>
            <m>\text{Thus, } z_{1} \cdot z_{2} = 12\left [ \text{cos}\left(\frac{5\pi}{6}\right) + i\text{sin}\left(\frac{5\pi}{6}\right) \right ] \text{ and } \frac{z_{1}}{z_{2}} = 3\left [ \text{cos}\left(\frac{\pi}{6}\right) + i\text{sin}\left(\frac{\pi}{6}\right) \right ]</m>
        </p>
    </solution>
</example>

<definition xml:id="def-argument-of-a-product">
    <statement>
        <p>
            <me>
                \textbf{Argument of a product}
            </me>
        </p>
        <p>
            The argument of the product of two complex numbers is the sum of their arguments.
        </p>
    </statement>
</definition>

<image source="/./media/image42.png" width="60%" />

<p>
    <m>\textbf{Proof:}</m>
</p>
<p>
    <m>\text{Let } z_{1} = r_{1}(\text{cos}\theta_{1} + i\text{sin}\theta_{1}) \ \ \ \text{and} \ \ \ z_{2} = r_{2}(\text{cos}\theta_{2} + i\text{sin}\theta_{2})</m>
</p>
<p>
    <m>\text{Now, } z_{1} \cdot z_{2} = r_{1}(\text{cos}\theta_{1} + i\text{sin}\theta_{1}) \cdot r_{2}(\text{cos}\theta_{2} + i\text{sin}\theta_{2})</m>
</p>
<p>
    <m> \ \ \ \ \ \ \ \ = r_{1} \cdot r_{2} \left [ \text{cos}\theta_{1}(\text{cos}\theta_{2} + i\text{sin}\theta_{2}) + i\text{sin}\theta_{1}(\text{cos}\theta_{2} + i\text{sin}\theta_{2}) \right ]</m>
</p>
<p>
    <m> \ \ \ \ \ \ \ \ = r_{1} \cdot r_{2} \left [ \text{cos}\theta_{1}\text{cos}\theta_{2} + i\text{cos}\theta_{1}\text{sin}\theta_{2} + i\text{sin}\theta_{1}\text{cos}\theta_{2} - \text{sin}\theta_{1}\text{sin}\theta_{2} \right ]</m>
</p>
<p>
    <m> \ \ \ \ \ \ \ \ = r_{1} \cdot r_{2} \left [ \text{cos}\theta_{1}\text{cos}\theta_{2} - \text{sin}\theta_{1}\text{sin}\theta_{2} + i(\text{cos}\theta_{1}\text{sin}\theta_{2} + \text{sin}\theta_{1}\text{cos}\theta_{2}) \right ]</m>
</p>
<p>
    <m> \ \ \ \ \ \ \ \ = \underline{\underline{ r_{1} \cdot r_{2} \left [ \text{cos}(\theta_{1} + \theta_{2}) + i\text{sin}(\theta_{1} + \theta_{2})\right ]}}</m>
</p>
<p>
    <m>\Rightarrow \text{arg} (z_{1} \cdot z_{2}) = \text{tan}^{-1} \left ( \frac{\text{sin}(\theta_{1} + \theta_{2})}{\text{cos}(\theta_{1} + \theta_{2})} \right )</m>
</p>
<p>
    <m> \ \ \ \ \ \ \ \ \ \ \ \ \ \ \ \ \ \ \ \ \ \ \ \ \ \ \ \ = \text{tan}^{-1} \left ( \text{tan}(\theta_{1} + \theta_{2}) \right )</m>
</p>
<p>
    <m> \ \ \ \ \ \ \ \ \ \ \ \ \ \ \ \ \ \ \ \ \ \ \ \ \ \ \ \ = \underline{\underline{ \theta_{1} + \theta_{2}}}</m>
</p>

<definition xml:id="def-argument-of-a-quotient">
    <statement>
        <p>
            <me>\textbf{Argument of the quotient}</me>
        </p>
        <p>
            The argument of the quotient of two complex numbers is the difference of their arguments.
        </p>
    </statement>
</definition>

<p>
    <m>\textbf{Proof:}</m>
</p>
<p>
    <m>\text{arg} \left ( \frac{z_{1}}{z_{2}} \right ) = \text{arg}(z_{1} \cdot {z_{2}}^{-1}) = \text{arg}(z_{1}) + (\text{arg} z_{2}^{-1}) = \text{arg}(z_{1}) + - (\text{arg} z_{2}) = \text{arg}(z_{1}) - \text{arg}(z_{2})</m>
</p>

<example>
    <statement>
        <p>
            <m> \text{arg} \left ( \frac{-4}{1 + \sqrt{3}\ i} \right ) = \text{arg}(-4) - \text{arg}(1 + \sqrt{3}\ i) = \pi - \frac{\pi}{3} = \frac{2\pi}{3}</m>
        </p>
    </statement>
</example>

<p>
    <me>
        \textbf{De Moivre's Formula}
    </me>
</p>
<p>
    Recall the product :<m>\ z_{1} \cdot z_{2} = r_{1} \cdot r_{2} \left [ \text{cos}(\theta_{1} + \theta_{2}) + i\text{sin}(\theta_{1} + \theta_{2})\right ]</m>.
</p>
<p>
    Similarly, we get <m>z_{1} \cdot z_{2} \cdots. z_{n} = r_{1} \cdot r_{2} \cdots. r_{n} \left [ \text{cos}(\theta_{1} + \theta_{2} + \cdots + \theta_{n}) + i\text{sin}(\theta_{1} + \theta_{2} + \cdots + \theta_{n})\right ]</m>.
</p>
<p>
    Now we can generalize that<m> z^{n} = r^{n} \left [ \text{cos}(\theta + \theta + \cdots + \theta) + i\text{sin}(\theta + \theta + \cdots + \theta)\right ]</m>.
</p>
<p>
    <m> \ \ \ \ \ \ \ \ \ \ \ \ \ \ \ \ \ \ = \underline{\underline{ r^{n} \left [ \text{cos}(n\theta) + i\text{sin}(n\theta)\right ]}}</m> which is called De Moivre's formula.
</p>

<example>
    <statement>
        <p>
            Express <m>(2 + 2i)^{100}</m> in polar form.
        </p>
    </statement>
    <solution>
        <p>
            <m>\text{Let } z = 2 + 2i. Then, r = \sqrt{8} , \ \ \theta = \frac{\pi}{4} </m> and hence
        </p>
        <p>
            <m>(2 + 2i)^{100} = z^{100}</m>
        </p>
        <p>
            <m> \ \ \ \ \ \ \ \ \ \ \ \ \ \ \ = \sqrt{8}^{100} \left [ \text{cos} 100 (\frac{\pi}{4}) + i\text{sin} 100 (\frac{\pi}{4})\right ]</m>
        </p>
        <p>
            <m> \ \ \ \ \ \ \ \ \ \ \ \ \ \ \ = \underline{\underline{ 8^{50} \left [ \text{cos}25\pi + i\text{sin}25\pi \right ]}}</m>
        </p>
    </solution>
</example>

<example>
    <statement>
        <p>
            Express <m>(\sqrt{3} + i)^{60}</m> in polar form.
        </p>
    </statement>
    <solution>
        <p>
            <m>\text{Let } z = \sqrt{3} + i. Then, r = 2 , \ \ \theta = \frac{\pi}{6} </m>.
        </p>
        <p>
            <m>\therefore (\sqrt{3} + i)^{60} = z^{60}</m>
        </p>
        <p>
            <m> \ \ \ \ \ \ \ \ \ \ \ \ \ \ \ = 2^{60} \left [ \text{cos} 60 (\frac{\pi}{6}) + i\text{sin} 60 (\frac{\pi}{6})\right ]</m>
        </p>
        <p>
            <m> \ \ \ \ \ \ \ \ \ \ \ \ \ \ \ = \underline{\underline{ 2^{60} \left [ \text{cos}10\pi + i\text{sin}10\pi \right ]}}</m>
        </p>
    </solution>
</example>

<definition xml:id="def-euler-s-formula">
    <statement>
        <p>
            <me>
                \textbf{Euler's formula}
            </me>
        </p>
        <p>
            The complex number <m>z = r(\text{cos}\theta + i\text{sin}\theta)</m> can be written in exponential form as: <m>z = re^{i\theta}</m> which is called Eulerâ€™s formula.
        </p>
    </statement>
</definition>
<p>
    <m>\text{Note:} \ \ \ \ z^{n} = r^{n} \left ( \text{cos}n \theta + i \text{sin}n\theta \right ) = r^{n} e^{{i}(n\theta)}</m>
</p>

<example>
    <statement>
        <p>
            <m>\text{Express the complex number } z = 1 + i \text{ using Euler's formula.}</m>
        </p>
    </statement>
    <solution>
        <p>
            <m> z = 1 + i</m>
        </p>
        <p>
            Now <m>r = \sqrt{2}</m> &amp; <m>\theta = \frac{\pi}{4} \Rightarrow z = re^{i\theta} = \underline{\underline{ \sqrt{2}e^{\frac{\pi i}{4}}}}</m>
        </p>
    </solution>
</example>
<example>
    <statement>
        <p>
            <m>\text{Express the complex number } z = 1 + \sqrt{3}i \text{ using Euler's formula.}</m>
        </p>
    </statement>
    <solution>
        <p>
            <m>z = 1 + \sqrt{3}i</m>
        </p>
        <p>
            Now <m>r = 2 </m> &amp; <m> \theta = \frac{\pi}{3} \Rightarrow z = re^{i\theta} = \underline{\underline{ 2e^{\frac{\pi i}{3}}}}</m>
        </p>
    </solution>
</example>
<example>
    <statement>
        <p>
            <m>\text{Express the complex number } z = (\sqrt{3} + i)^{7} \text{ using Euler's formula.}</m>
        </p>
    </statement>
    <solution>
        <p>
            <m>z = (\sqrt{3} + i)^{7}</m>
        </p>
        <p>
            Now <m>r = 2 </m> &amp; <m> \theta = \frac{\pi}{6} \Rightarrow z = re^{i\theta} = 2^{7}e^{\frac{7\pi i}{6}} = 128e^{\frac{7\pi i}{6}}</m>
        </p>
    </solution>
</example>


<exercise><stack source="/questions/top/Mathematics-for-NS-&amp;-SS-23-24-Question-Bank/The-Real-and-Complex-Number-Systems-(NS)/Polar-form-of-a-complex-number/Converting-Complex-Numbers-Rectangular-to-Polar-Form.xml" /></exercise>
<exercise><stack source="/questions/top/Mathematics-for-NS-&amp;-SS-23-24-Question-Bank/The-Real-and-Complex-Number-Systems-(NS)/Polar-form-of-a-complex-number/Conversion-to-Polar-Form-Complex-Number-z-=-x-+-yi.xml" /></exercise>
</subsection>

